theories/case_studies/dle/deep_locality_spec.v
@@ -1,6 +1,6 @@
 From iris.proofmode Require Import proofmode.
 From cap_machine Require Import region_invariants_allocation region_invariants_revocation interp_weakening monotone.
-From cap_machine Require Import rules logrel logrel_extra monotone register_tactics.
+From cap_machine Require Import rules logrel world_interp_stack monotone register_tactics.
 From cap_machine Require Import fetch_spec assert_spec switcher_spec_call deep_locality.
 From cap_machine Require Import world_ghost_theory world_ghost_theory_interface.
 From cap_machine Require Import proofmode.
